fv/lean/Ragu/Instances/Point/Alloc.lean
@@ -1,4 +1,3 @@
-import Clean.Circuit
 import Ragu.Circuits.Point.Alloc
 import Ragu.Core
 
@@ -8,7 +7,7 @@ open Core.Primes
 @[reducible]
 def CircuitField := F Core.Primes.p
 
-def operations : Operations CircuitField := [
+def exported_operations : Operations CircuitField := [
   Operation.witness 3 (fun _env => default),
   Operation.assert ((((var 0) * (var 1)) + (0x40000000000000000000000000000000224698fc094cf91b992d30ed00000000 * (var 2)))),
   Operation.assert (((var 0) + (0x40000000000000000000000000000000224698fc094cf91b992d30ed00000000 * (var 1)))),
@@ -22,10 +21,12 @@ def operations : Operations CircuitField := [
   Operation.assert ((((var 5) + (0x0000000000000000000000000000000000000000000000000000000000000005 * 1)) + (0x40000000000000000000000000000000224698fc094cf91b992d30ed00000000 * (var 8)))),
 ]
 
+def output : List (Expression CircuitField) := [(var 0), (var 6)]
+
 def circuit := Circuits.Point.Alloc.circuit.main (F:=CircuitField) default
 
-
-theorem same_circuit : (circuit.operations 0).toFlat = operations.toFlat :=  by
+theorem same_circuit :
+    (circuit.operations 0).toFlat = exported_operations.toFlat := by
   simp [Operations.toFlat, circuit_norm, FormalCircuit.toSubcircuit,
     circuit,
     Circuits.Point.Alloc.circuit, Circuits.Point.Alloc.elaborated, Circuits.Point.Alloc.main,
@@ -33,5 +34,17 @@ theorem same_circuit : (circuit.operations 0).toFlat = operations.toFlat :=  by
     Circuits.Element.AllocSquare.circuit, Circuits.Element.AllocSquare.elaborated, Circuits.Element.AllocSquare.main,
     Circuits.Element.Mul.circuit, Circuits.Element.Mul.elaborated, Circuits.Element.Mul.main]
   rfl
+
+theorem same_output :
+    (circuit.output 0).x = output[0] ∧
+    (circuit.output 0).y = output[1] := by
+  simp [circuit_norm,
+    circuit, output,
+    Circuits.Point.Alloc.circuit, Circuits.Point.Alloc.elaborated, Circuits.Point.Alloc.main,
+    Circuits.Core.AllocMul.circuit, Circuits.Core.AllocMul.elaborated, Circuits.Core.AllocMul.main,
+    Circuits.Element.AllocSquare.circuit, Circuits.Element.AllocSquare.elaborated, Circuits.Element.AllocSquare.main,
+    Circuits.Element.Mul.circuit, Circuits.Element.Mul.elaborated, Circuits.Element.Mul.main]
+  constructor <;> rfl
+
 
 end Ragu.Instances.Point.Alloc
